regex/Regex/Backtracker/Basic.lean
@@ -1,96 +1,88 @@
 import Regex.Data.BitMatrix
-import Regex.Data.BoundedIterator
+import Regex.Data.BVPos
 import Regex.NFA
 import Regex.Strategy
 
-open String (Iterator Pos)
-open Regex.Data (BitMatrix BoundedIterator)
+open String (ValidPos)
+open Regex.Data (BitMatrix BVPos)
 
 set_option autoImplicit false
 
 namespace Regex.Backtracker
 
-structure StackEntry (σ : Strategy) (nfa : NFA) (startIdx maxIdx : Nat) where
+structure StackEntry {s : String} (σ : Strategy s) (nfa : NFA) (startPos : ValidPos s) where
   update : σ.Update
   state : Fin nfa.nodes.size
-  it : BoundedIterator startIdx maxIdx
+  pos : BVPos startPos
 
-def captureNextAux.pushNext (σ : Strategy) (nfa : NFA) (wf : nfa.WellFormed) (startIdx maxIdx : Nat) (stack : List (StackEntry σ nfa startIdx maxIdx))
-  (update : σ.Update) (state : Fin nfa.nodes.size) (it : BoundedIterator startIdx maxIdx) :
-  List (StackEntry σ nfa startIdx maxIdx) :=
+def captureNextAux.pushNext {s : String} (σ : Strategy s) (nfa : NFA) (wf : nfa.WellFormed) (startPos : ValidPos s) (stack : List (StackEntry σ nfa startPos))
+  (update : σ.Update) (state : Fin nfa.nodes.size) (pos : BVPos startPos) :
+  List (StackEntry σ nfa startPos) :=
   match hn : nfa[state] with
   | .done => stack
   | .fail => stack
   | .epsilon state' =>
     have isLt : state' < nfa.nodes.size := wf.inBounds' state hn
-    ⟨update, ⟨state', isLt⟩, it⟩ :: stack
+    ⟨update, ⟨state', isLt⟩, pos⟩ :: stack
   | .split state₁ state₂ =>
     have isLt : state₁ < nfa.nodes.size ∧ state₂ < nfa.nodes.size := wf.inBounds' state hn
-    ⟨update, ⟨state₁, isLt.1⟩, it⟩ :: ⟨update, ⟨state₂, isLt.2⟩, it⟩ :: stack
+    ⟨update, ⟨state₁, isLt.1⟩, pos⟩ :: ⟨update, ⟨state₂, isLt.2⟩, pos⟩ :: stack
   | .save offset state' =>
     have isLt : state' < nfa.nodes.size := wf.inBounds' state hn
-    let update' := σ.write update offset it.pos
-    ⟨update', ⟨state', isLt⟩, it⟩ :: stack
+    let update' := σ.write update offset pos.current
+    ⟨update', ⟨state', isLt⟩, pos⟩ :: stack
   | .anchor a state' =>
     have isLt : state' < nfa.nodes.size := wf.inBounds' state hn
-    if a.test it.it then
-      ⟨update, ⟨state', isLt⟩, it⟩ :: stack
+    if a.test pos.current then
+      ⟨update, ⟨state', isLt⟩, pos⟩ :: stack
     else
       stack
   | .char c state' =>
     have isLt : state' < nfa.nodes.size := wf.inBounds' state hn
-    if h : ∃ hnext : it.hasNext, it.curr hnext = c then
-      ⟨update, ⟨state', isLt⟩, it.next h.1⟩ :: stack
+    if h : ∃ h : pos ≠ s.endBVPos startPos, pos.get h = c then
+      ⟨update, ⟨state', isLt⟩, pos.next h.1⟩ :: stack
     else
       stack
   | .sparse cs state' =>
     have isLt : state' < nfa.nodes.size := wf.inBounds' state hn
-    if h : ∃ hnext : it.hasNext, it.curr hnext ∈ cs then
-      ⟨update, ⟨state', isLt⟩, it.next h.1⟩ :: stack
+    if h : ∃ h : pos ≠ s.endBVPos startPos, pos.get h ∈ cs then
+      ⟨update, ⟨state', isLt⟩, pos.next h.1⟩ :: stack
     else
       stack
 
-def captureNextAux (σ : Strategy) (nfa : NFA) (wf : nfa.WellFormed) (startIdx maxIdx : Nat)
-  (visited : BitMatrix nfa.nodes.size (maxIdx + 1 - startIdx)) (stack : List (StackEntry σ nfa startIdx maxIdx)) :
-  (Option σ.Update × BitMatrix nfa.nodes.size (maxIdx + 1 - startIdx)) :=
+def captureNextAux {s : String} (σ : Strategy s) (nfa : NFA) (wf : nfa.WellFormed) (startPos : ValidPos s)
+  (visited : BitMatrix nfa.nodes.size (startPos.remainingBytes + 1)) (stack : List (StackEntry σ nfa startPos)) :
+  (Option σ.Update × BitMatrix nfa.nodes.size (startPos.remainingBytes + 1)) :=
   match stack with
   | [] => (.none, visited)
-  | ⟨update, state, it⟩ :: stack' =>
-    if h : visited.get state it.index then
-      captureNextAux σ nfa wf startIdx maxIdx visited stack'
+  | ⟨update, state, pos⟩ :: stack' =>
+    if h : visited.get state pos.index then
+      captureNextAux σ nfa wf startPos visited stack'
     else
-      let visited' := visited.set state it.index
-      have : nfa.nodes.size * (maxIdx + 1 - startIdx) + 1 - visited'.popcount < nfa.nodes.size * (maxIdx + 1 - startIdx) + 1 - visited.popcount :=
-        BitMatrix.popcount_decreasing visited state it.index h
+      let visited' := visited.set state pos.index
+      have : nfa.nodes.size * (startPos.remainingBytes + 1) + 1 - visited'.popcount < nfa.nodes.size * (startPos.remainingBytes + 1) + 1 - visited.popcount :=
+        BitMatrix.popcount_decreasing visited state pos.index h
       if nfa[state].isDone then
         (.some update, visited')
       else
-        let stack'' := captureNextAux.pushNext σ nfa wf startIdx maxIdx stack' update state it
-        captureNextAux σ nfa wf startIdx maxIdx visited' stack''
-termination_by (nfa.nodes.size * (maxIdx + 1 - startIdx) + 1 - visited.popcount, stack)
+        let stack'' := captureNextAux.pushNext σ nfa wf startPos stack' update state pos
+        captureNextAux σ nfa wf startPos visited' stack''
+termination_by (nfa.nodes.size * (startPos.remainingBytes + 1) + 1 - visited.popcount, stack)
 
-def captureNext (σ : Strategy) (nfa : NFA) (wf : nfa.WellFormed) (it : Iterator) : Option σ.Update :=
-  let startIdx := it.pos.byteIdx
-  let maxIdx := it.toString.endPos.byteIdx
-  if le : it.pos ≤ it.toString.endPos then
-    let bit : BoundedIterator startIdx maxIdx := ⟨it, Nat.le_refl _, le, rfl⟩
-    go startIdx maxIdx bit (BitMatrix.zero _ _)
-  else
-    .none
+def captureNext {s : String} (σ : Strategy s) (nfa : NFA) (wf : nfa.WellFormed) (startPos : ValidPos s) : Option σ.Update :=
+  go (.refl startPos) (BitMatrix.zero _ _)
 where
-  go (startIdx maxIdx : Nat) (bit : BoundedIterator startIdx maxIdx) (visited : BitMatrix nfa.nodes.size (maxIdx + 1 - startIdx)) :
-  Option σ.Update :=
-  match captureNextAux σ nfa wf startIdx maxIdx visited [⟨σ.empty, ⟨nfa.start, wf.start_lt⟩, bit⟩] with
+  go (pos : BVPos startPos) (visited : BitMatrix nfa.nodes.size (startPos.remainingBytes + 1)) : Option σ.Update :=
+  match captureNextAux σ nfa wf startPos visited [⟨σ.empty, ⟨nfa.start, wf.start_lt⟩, pos⟩] with
   | (.some update, _) => .some update
   | (.none, visited') =>
-    if h : bit.hasNext then
-      have : (bit.next h).remainingBytes < bit.remainingBytes := bit.next_remainingBytes_lt h
-      go startIdx maxIdx (bit.next h) visited'
+    if h : pos ≠ s.endBVPos startPos then
+      go (pos.next h) visited'
     else
       .none
-  termination_by bit.remainingBytes
+  termination_by pos
 
-def captureNextBuf (nfa : NFA) (wf : nfa.WellFormed) (bufferSize : Nat) (it : Iterator) : Option (Buffer bufferSize) :=
-  captureNext (BufferStrategy bufferSize) nfa wf it
+def captureNextBuf {s : String} (nfa : NFA) (wf : nfa.WellFormed) (bufferSize : Nat) (p : ValidPos s) : Option (Buffer s bufferSize) :=
+  captureNext (BufferStrategy s bufferSize) nfa wf p
 
 end Regex.Backtracker
