regex/Regex/Data/BVPos.lean
@@ -1,0 +1,80 @@
+import Regex.Data.String
+
+set_option autoImplicit false
+
+open String (ValidPos)
+
+namespace Regex.Data
+
+/--
+A valid position in a string with a lower bound.
+-/
+@[ext]
+structure BVPos {s : String} (startPos : ValidPos s) where
+  current : ValidPos s
+  le : startPos ≤ current
+deriving DecidableEq
+
+def _root_.String.endBVPos (s : String) (startPos : ValidPos s) : BVPos startPos :=
+  ⟨s.endValidPos, startPos.isValid.le_rawEndPos⟩
+
+namespace BVPos
+
+variable {s : String} {startPos : ValidPos s}
+
+def refl {s : String} (startPos : ValidPos s) : BVPos startPos :=
+  ⟨startPos, ValidPos.le_refl _⟩
+
+def index (bp : BVPos startPos) : Fin (startPos.remainingBytes + 1) :=
+  have lt : startPos.offset.byteDistance bp.current.offset < startPos.remainingBytes + 1 := by
+    simp only [String.Pos.Raw.byteDistance, ValidPos.remainingBytes_eq]
+    have : bp.current.offset.byteIdx ≤ s.utf8ByteSize := bp.current.isValid.le_rawEndPos
+    grind
+  ⟨startPos.offset.byteDistance bp.current.offset, lt⟩
+
+theorem ne_iff_current_ne {bp₁ bp₂ : BVPos startPos} : bp₁ ≠ bp₂ ↔ bp₁.current ≠ bp₂.current := by
+  grind [BVPos.ext]
+
+theorem ne_end_iff_current_ne_end {bp : BVPos startPos} : bp ≠ s.endBVPos startPos ↔ bp.current ≠ s.endValidPos := by
+  simp [ne_iff_current_ne, String.endBVPos]
+
+def next (bp : BVPos startPos) (h : bp ≠ s.endBVPos startPos) : BVPos startPos :=
+  let current' := bp.current.next (ne_end_iff_current_ne_end.mp h)
+  have le' : startPos ≤ current' := ValidPos.le_of_lt (Nat.lt_of_le_of_lt bp.le bp.current.lt_next)
+  ⟨current', le'⟩
+
+def nextn (bp : BVPos startPos) (n : Nat) : BVPos startPos :=
+  match n with
+  | 0 => bp
+  | n + 1 =>
+    if h : bp ≠ s.endBVPos startPos then
+      nextn (bp.next h) n
+    else
+      bp
+
+def get (bp : BVPos startPos) (h : bp ≠ s.endBVPos startPos) : Char :=
+  bp.current.get (ne_end_iff_current_ne_end.mp h)
+
+def lt (bp₁ bp₂ : BVPos startPos) : Prop := bp₁.current < bp₂.current
+
+instance : LT (BVPos startPos) := ⟨lt⟩
+
+@[simp]
+theorem lt_next {bp : BVPos startPos} (h : bp ≠ s.endBVPos startPos) : bp < bp.next h :=
+  bp.current.lt_next (h := ne_end_iff_current_ne_end.mp h)
+
+theorem wellFounded_lt : WellFounded (fun (p : BVPos startPos) q => q < p) :=
+  InvImage.wf BVPos.current ValidPos.wellFounded_gt
+
+instance : WellFoundedRelation (BVPos startPos) where
+  rel p q := q < p
+  wf := wellFounded_lt
+
+end BVPos
+
+end Regex.Data
+
+-- From Init.Data.String.Termination
+macro_rules | `(tactic| decreasing_trivial) => `(tactic|
+  (with_reducible change (_ : Regex.Data.BVPos _) < _
+   simp) <;> done)
